

Two-Body Partial Derivatives

This document is a compilation of partial derivatives of the astrodynamic two-body problem. Partial derivatives are summarized for circular, elliptical and hyperbolic two-body motion.

Downstream error propagation derivatives for a circular orbit

$$\frac{\partial v_f}{\partial v} = 2 \cos \theta_f - 1$$

$$\frac{\partial r_f}{\partial v} = \frac{2r_i}{v_i} (1 - \cos \theta_f)$$

$$\frac{\partial \gamma_f}{\partial v} = \frac{2}{v_i} \sin \theta_f$$

$$\frac{\partial \theta_f}{\partial v} = \frac{1}{v_i} (4 \sin \theta_f - 3 \theta_f)$$

$$\frac{\partial v_f}{\partial \gamma} = -v_i \sin \theta_f$$

$$\frac{\partial r_f}{\partial \gamma} = r_i \sin \theta_f$$

$$\frac{\partial \gamma_f}{\partial \gamma} = \cos \theta_f$$

$$\frac{\partial \theta_f}{\partial \gamma} = -2(1 - \cos \theta_f)$$

where

r_i = initial position magnitude

r_f = final position magnitude

v_i = initial velocity magnitude = $\sqrt{\mu/r_i}$

v_f = final velocity magnitude

θ_f = final true anomaly

γ_f = final flight path angle

μ = gravitational constant

Elliptical orbits

apoapsis radius with respect to r, v, γ

$$\frac{\partial r_a}{\partial r} = \frac{(1+e \cos \theta)(1+e)}{(1-e^2)^2} \{2+e-e^2+\cos \theta+e \cos \theta\}$$

$$\frac{\partial r_a}{\partial v} = \frac{2a^{\frac{3}{2}}(1+2e+e^2)(1+\cos \theta)}{\sqrt{\mu}(1-e^2)^{\frac{1}{2}}(1+2e \cos \theta+e^2)^{\frac{1}{2}}}$$

$$\frac{\partial r_a}{\partial \gamma} = \frac{a(1-e^2) \sin \theta}{1+e \cos \theta}$$

periapsis radius with respect to r, v, γ

$$\frac{\partial r_p}{\partial r} = \frac{(1+e \cos \theta)(1+e)}{(1-e^2)^2} \{2-e-e^2-\cos \theta-e \cos \theta\}$$

$$\frac{\partial r_p}{\partial v} = \frac{2a^{\frac{3}{2}}(1-2e+e^2)(1-\cos \theta)}{\sqrt{\mu}(1-e^2)^{\frac{1}{2}}(1+2e \cos \theta+e^2)^{\frac{1}{2}}}$$

$$\frac{\partial r_p}{\partial \gamma} = \frac{-a(1-e^2) \sin \theta}{1+e \cos \theta}$$

orbital period with respect to r, v, γ

$$\frac{\partial \tau}{\partial r} = \frac{3\tau a}{r^2} \quad \frac{\partial \tau}{\partial v} = \frac{3\tau(2a-r)}{rv} = \frac{3av\tau}{\mu} \quad \frac{\partial \tau}{\partial \gamma} = 0$$

true anomaly with respect to r, v, γ

$$\frac{\partial \theta}{\partial r} = -\frac{\sin \theta(1+e \cos \theta)}{ae(1-e^2)}$$

$$\frac{\partial \theta}{\partial v} = -\frac{2 \sin \theta}{e} \left\{ \frac{a(1-e^2)}{\mu(1+2e \cos \theta+e^2)} \right\}^{\frac{1}{2}}$$

$$\frac{\partial \theta}{\partial \gamma} = 2 + \frac{(1-e^2)}{e} \left\{ \frac{\cos \theta}{1+e \cos \theta} \right\}$$

orbital eccentricity with respect to r, v, γ

$$\frac{\partial e}{\partial r} = \frac{v^2 \cos^2 \gamma}{\mu e a} (a - r) = \frac{e + \cos \theta}{r}$$

$$\frac{\partial e}{\partial v} = \frac{2rv \cos^2 \gamma}{\mu e a} (a - r)$$

$$\frac{\partial e}{\partial \gamma} = \frac{r^2 v^2 \sin 2\gamma}{2\mu e a}$$

semimajor axis with respect to r, v, γ

$$\frac{\partial a}{\partial r} = \frac{2a^2}{r^2} \quad \frac{\partial a}{\partial v} = \frac{2a^2 v}{\mu} \quad \frac{\partial a}{\partial \gamma} = 0$$

semimajor axis, eccentricity, orbital period and apogee radius with respect to periapsis radius

$$\frac{\partial a}{\partial r_p} = 2 \left\{ \frac{r_a}{r_p (1+e)} \right\}^2 = 2 \left(\frac{a}{r_p} \right)^2 = \frac{2(1+e \cos \theta)^2}{(1-e^2)^2}$$

$$\frac{\partial e}{\partial r_p} = \frac{e + \cos \theta}{r_p}$$

$$\frac{\partial \tau}{\partial r_p} = \frac{3\tau a}{r_p^2}$$

$$\frac{\partial r_a}{\partial r_p} = \frac{(1+e \cos \theta)(2 + \cos \theta - e)}{(1-e)^2}$$

semimajor axis, eccentricity, orbital period and apogee radius with respect to periapsis velocity

$$\frac{\partial a}{\partial v_p} = \frac{2a(2a - r_p)}{r_p v_p}$$

$$\frac{\partial e}{\partial v_p} = \frac{2(e + \cos \theta)}{v_p}$$

$$\frac{\partial \tau}{\partial v_p} = \frac{3\tau(2a - r_p)}{r_p v_p}$$

$$\frac{\partial r_a}{\partial v_p} = \frac{2a(1 + \cos \theta)(1 + e)}{v_p(1 - e)}$$

where

r = position magnitude

v = velocity magnitude

γ = flight path angle

θ = true anomaly

e = orbital eccentricity

r_p = periapsis radius

r_a = apoapsis radius

a = semimajor axis

τ = orbital period

In the following series of equations, \mathbf{x} represents the Cartesian state vector consisting of position vector \mathbf{r} , and velocity vector \mathbf{v} .

position vector

$$\frac{\partial \mathbf{r}}{\partial \mathbf{x}} = \begin{bmatrix} \mathbf{r}^T / r & \mathbf{0} \end{bmatrix}$$

velocity vector

$$\frac{\partial \mathbf{v}}{\partial \mathbf{x}} = \begin{bmatrix} \mathbf{0} & \mathbf{v}^T / v \end{bmatrix}$$

angular momentum vector

$$\frac{\partial \mathbf{h}}{\partial \mathbf{x}} = \begin{bmatrix} \mathbf{I} \times \mathbf{v} & \mathbf{r} \times \mathbf{I} \end{bmatrix}$$

angular momentum magnitude

$$\frac{\partial h}{\partial \mathbf{x}} = \begin{bmatrix} \mathbf{h}^T (\mathbf{I} \times \mathbf{v}) / h & \mathbf{h}^T (\mathbf{r} \times \mathbf{I}) / h \end{bmatrix}$$

eccentricity vector

$$\frac{\partial \mathbf{e}}{\partial \mathbf{x}} = \begin{bmatrix} (v^2 / \mu - 1 / r) \mathbf{I} + \mathbf{r} \mathbf{r}^T / r^3 - \mathbf{v} \mathbf{v}^T / \mu & 2 \mathbf{r} \mathbf{v}^T / \mu - (\mathbf{v} \cdot \mathbf{r}) \mathbf{I} / \mu - \mathbf{v} \mathbf{r}^T / \mu \end{bmatrix}$$

specific orbital energy

$$\frac{\partial C_3}{\partial \mathbf{x}} = \begin{bmatrix} 2 \mu \mathbf{r}^T / r^3 & 2 \mathbf{v}^T \end{bmatrix}$$

sine of flight path angle

$$\frac{\partial \sin \gamma}{\partial \mathbf{x}} = \begin{bmatrix} \hat{\mathbf{v}}^T (\mathbf{I}/r - \mathbf{r}\mathbf{r}^T/r^3) & \hat{\mathbf{r}}^T (\mathbf{I}/v - \mathbf{v}\mathbf{v}^T/v^3) \end{bmatrix}$$

semimajor axis

$$\frac{\partial a}{\partial \mathbf{r}} = \frac{2a^2 \mathbf{r}}{r^3} \quad \frac{\partial a}{\partial \mathbf{v}} = \frac{2a^2 \mathbf{v}}{\mu}$$

where

$$\mathbf{r} = [r_x, r_y, r_z]^T = \text{position vector}$$

$$r = |\mathbf{r}| = \text{position magnitude}$$

$$\mathbf{v} = [v_x, v_y, v_z]^T = \text{velocity vector}$$

$$v = |\mathbf{v}| = \text{velocity magnitude}$$

$$\mathbf{h} = \mathbf{r} \times \mathbf{v} = [h_x, h_y, h_z]^T = \text{angular momentum vector}$$

$$h = |\mathbf{r} \times \mathbf{v}| = \text{angular momentum magnitude}$$

$$\mathbf{e} = \text{orbital eccentricity vector}$$

$$\mathbf{I} = \begin{bmatrix} 1 & 0 & 0 \\ 0 & 1 & 0 \\ 0 & 0 & 1 \end{bmatrix} = \text{identity matrix}$$

Hyperbolic orbits

In the following series of equations, \mathbf{x} represents the state vector consisting of position vector \mathbf{r} , and velocity \mathbf{v} . C_3 is equal to twice the specific (per unit mass) orbital energy.

scaled unit asymptote vector

$$\begin{aligned} \frac{\partial \tilde{\mathbf{s}}}{\partial \mathbf{x}} &= C_3 \frac{\partial \hat{\mathbf{s}}}{\partial \mathbf{x}} + \hat{\mathbf{s}} \frac{\partial C_3}{\partial \mathbf{x}} \\ &= \frac{\sqrt{C_3^3}}{\mu e^2} \left\{ \left(\frac{\partial \mathbf{h}}{\partial \mathbf{x}} \times \mathbf{e} \right) + \left(\mathbf{h} \times \frac{\partial \mathbf{e}}{\partial \mathbf{x}} \right) \right\} - \frac{C_3}{e^2} \frac{\partial \mathbf{e}}{\partial \mathbf{x}} + \left\{ \frac{3}{2C_3} \frac{\partial C_3}{\partial \mathbf{x}} - \frac{2}{e^2} \left(\mathbf{e} \cdot \frac{\partial \mathbf{e}}{\partial \mathbf{x}} \right) \right\} \tilde{\mathbf{s}} + \frac{1}{2e^2} \frac{\partial C_3}{\partial \mathbf{x}} \mathbf{e} \end{aligned}$$

The asymptote unit vector of a hyperbolic orbit is given by

$$\hat{\mathbf{s}} = \begin{Bmatrix} \cos \delta_{\infty} \cos \alpha_{\infty} \\ \cos \delta_{\infty} \sin \alpha_{\infty} \\ \sin \delta_{\infty} \end{Bmatrix}$$

In this expression, α_{∞} is the right ascension of the asymptote (RLA), and δ_{∞} is the declination of the asymptote (DLA).

The asymptote unit vector at any trajectory time can also be computed from

$$\hat{\mathbf{s}} = \frac{1}{1 + C_3 \frac{h^2}{\mu^2}} \left\{ \left(\frac{\sqrt{C_3}}{\mu} \right) \mathbf{h} \times \mathbf{e} - \mathbf{e} \right\} = \frac{1}{1 + C_3 \frac{p}{\mu}} \left\{ \left(\frac{\sqrt{C_3}}{\mu} \right) \mathbf{h} \times \mathbf{e} - \mathbf{e} \right\}$$

where p is the semi-parameter of the orbit.